fixed the 3rd issue in r3967.
All the rest problems are about updating typing rules (ordered by
complexity).

1) The current rules still check if variables used in unreachable blocks
are well-typed. W.r.t r3970, we should ignore checking anything in
unreachable blocks. But, this may break a lot of proofs globally, because almost
all well-formnedss inversion lemma will require reachability conditions
after the change.

2) the 5th problem in r3964, equivalence of two CFG functions

3) a) the 3rd problem in r3962, hoisting dom-analysis on the top of a
function under check.
   b) hoisting layouts checking on the top of a checked module.

4) wf_const_gid should check fdec



git-svn-id: https://webdav.seas.upenn.edu/svn/sol/vol@3971 eef5ea85-cc2e-0410-bd84-0fae1f012da8

src3.0/Transforms/mem2reg_correct.v
@@ -58,6 +58,10 @@ Proof.
   eapply program_sim_trans; eauto.
 Qed.
 
+Lemma subst_fdef_PI_f__PI_f_subst_pinfo: forall i1 v pinfo,
+  subst_fdef i1 v (PI_f pinfo) = PI_f (subst_pinfo i1 v pinfo).
+Proof. destruct pinfo; auto. Qed.
+
 Lemma las_die_wfPI: forall (los : layouts) (nts : namedts) (fh : fheader)
   (dones : list id) (pinfo: PhiInfo)
   (bs1 : list block) (l0 : l) (ps0 : phinodes) (cs0 : cmds) (tmn0 : terminator)
@@ -74,7 +78,7 @@ Lemma las_die_wfPI: forall (los : layouts) (nts : namedts) (fh : fheader)
           product_fdef
             (fdef_intro fh (bs1 ++ block_intro l0 ps0 cs0 tmn0 :: bs2))
           :: Ps2)]),
-  WF_PhiInfo (update_pinfo pinfo
+  WF_PhiInfo (update_pinfo (subst_pinfo i1 v pinfo)
          (fdef_intro fh
            (List.map (remove_block i1)
              (List.map (subst_block i1 v)
@@ -94,21 +98,10 @@ Proof.
   assert (Hdiinfo:=HwfS).
   eapply las_diinfo in Hdiinfo; eauto.
   destruct Hdiinfo as [diinfo [J1 J2]]. rewrite Heq in J1.
-  change
-    (update_pinfo pinfo
-      (remove_fdef i1
-        (subst_fdef i1 v
-          (fdef_intro fh (bs1 ++ block_intro l0 ps0 cs0 tmn0 :: bs2))))) with
-    (update_pinfo
-      (update_pinfo pinfo
-        (subst_fdef i1 v
-          (fdef_intro fh (bs1 ++ block_intro l0 ps0 cs0 tmn0 :: bs2))))
-      (remove_fdef i1
-        (subst_fdef i1 v
-          (fdef_intro fh (bs1 ++ block_intro l0 ps0 cs0 tmn0 :: bs2))))).
   eapply die_wfPI; eauto.
     eapply las_wfPI; eauto.
     eapply las_wfS; eauto.
+    rewrite <- Heq. apply subst_fdef_PI_f__PI_f_subst_pinfo.
 Qed.
 
 Lemma las_die_sim_wfS: forall (los : layouts) (nts : namedts) (fh : fheader)
@@ -187,7 +180,7 @@ Lemma laa_die_wfPI: forall (los : layouts) (nts : namedts) (fh : fheader)
           product_fdef
             (fdef_intro fh (bs1 ++ block_intro l0 ps0 cs0 tmn0 :: bs2))
           :: Ps2)]),
-  WF_PhiInfo (update_pinfo pinfo
+  WF_PhiInfo (update_pinfo (subst_pinfo i1 v pinfo)
     (fdef_intro fh
       (List.map (remove_block i1)
         (List.map (subst_block i1 v)
@@ -207,21 +200,10 @@ Proof.
   assert (Hdiinfo:=HwfS).
   eapply laa_diinfo in Hdiinfo; eauto.
   destruct Hdiinfo as [diinfo [J1 J2]]. rewrite Heq in J1.
-  change
-    (update_pinfo pinfo
-      (remove_fdef i1
-        (subst_fdef i1 v
-          (fdef_intro fh (bs1 ++ block_intro l0 ps0 cs0 tmn0 :: bs2))))) with
-    (update_pinfo
-      (update_pinfo pinfo
-        (subst_fdef i1 v
-          (fdef_intro fh (bs1 ++ block_intro l0 ps0 cs0 tmn0 :: bs2))))
-      (remove_fdef i1
-        (subst_fdef i1 v
-          (fdef_intro fh (bs1 ++ block_intro l0 ps0 cs0 tmn0 :: bs2))))).
   eapply die_wfPI; eauto.
     eapply laa_wfPI; eauto.
     eapply laa_wfS; eauto.
+    rewrite <- Heq. apply subst_fdef_PI_f__PI_f_subst_pinfo.
 Qed.
 
 Lemma laa_die_sim_wfS: forall (los : layouts) (nts : namedts) (fh : fheader)
@@ -324,6 +306,26 @@ Proof.
       split; auto.
 Qed.
 
+Definition keep_pinfo (f:fdef) (pinfo1 pinfo2: PhiInfo) :=
+PI_f pinfo2 = f /\
+PI_id pinfo1 = PI_id pinfo2 /\
+PI_typ pinfo1 = PI_typ pinfo2 /\
+PI_align pinfo1 = PI_align pinfo2.
+
+Hint Unfold keep_pinfo.
+
+Ltac instantiate_pinfo :=
+match goal with
+| HwfS : WF_PhiInfo (update_pinfo ?f ?pi) |- _ => 
+  exists (update_pinfo f pi); split; auto
+| HwfS : WF_PhiInfo ?pi, Heq: (PI_f ?pi) = ?f |- 
+  exists _ : _, WF_PhiInfo _ /\ keep_pinfo ?f ?pi _ =>
+  rewrite <- Heq; exists pi; split; auto
+| HwfS : WF_PhiInfo ?pi |- 
+  exists _ : _, WF_PhiInfo _ /\ keep_pinfo (PI_f ?pi) ?pi _ =>
+  exists pi; split; auto
+end.
+
 Lemma elim_stld_cmds_wfPI: forall los nts fh dones (pinfo:PhiInfo) f0 dones0
   bs1 l0 ps0 cs0 tmn0 bs2 Ps1 Ps2
   (Hpass : (f0, true, dones0) =
@@ -339,23 +341,23 @@ Lemma elim_stld_cmds_wfPI: forall los nts fh dones (pinfo:PhiInfo) f0 dones0
           product_fdef
             (fdef_intro fh (bs1 ++ block_intro l0 ps0 cs0 tmn0 :: bs2))
           :: Ps2)]),
-  WF_PhiInfo (update_pinfo pinfo f0).
+  exists pinfo', WF_PhiInfo pinfo' /\ keep_pinfo f0 pinfo pinfo'.
 Proof.
   intros.
   unfold elim_stld_cmds in Hpass.
   remember (find_init_stld cs0 (PI_id pinfo) dones) as R1.
   destruct R1 as [[[[]]|[]]|]; tinv Hpass.
     remember (find_next_stld c (PI_id pinfo)) as R2.
-    destruct R2 as [[|[]]|]; inv Hpass.
-      eapply las_die_wfPI; eauto.
-      eapply sas_wfPI; eauto.
-      rewrite <- Heq. rewrite update_pinfo_eq; auto.
+    destruct R2 as [[|[]]|]; inv Hpass; eauto.
+      eapply las_die_wfPI in HwfS; eauto. instantiate_pinfo.
+      eapply sas_wfPI in HwfS; eauto. instantiate_pinfo.
+      instantiate_pinfo.
 
     remember (find_next_stld c (PI_id pinfo)) as R2.
     destruct R2 as [[|[]]|]; inv Hpass.
-      eapply laa_die_wfPI; eauto.
-      rewrite <- Heq. rewrite update_pinfo_eq; auto.
-      rewrite <- Heq. rewrite update_pinfo_eq; auto.
+      eapply laa_die_wfPI in HwfS; eauto. instantiate_pinfo.
+      instantiate_pinfo.
+      instantiate_pinfo.
 Qed.
 
 Lemma elim_stld_cmds_sim_wfS: forall los nts fh dones (pinfo:PhiInfo) f0 dones0
@@ -434,11 +436,10 @@ Lemma elim_stld_blocks_wfPI_aux: forall los nts fh dones (pinfo:PhiInfo) f0
          (Ps1 ++
           product_fdef
             (fdef_intro fh (bs1 ++ bs2)) :: Ps2)]),
-  WF_PhiInfo (update_pinfo pinfo f0).
+  exists pinfo', WF_PhiInfo pinfo' /\ keep_pinfo f0 pinfo pinfo'.
 Proof.
   induction bs2; simpl; intros.
-    inv Hpass.
-    rewrite <- Heq. rewrite update_pinfo_eq; auto.
+    inv Hpass. instantiate_pinfo.
 
     destruct a as [l0 ps0 cs0 tmn0].
     remember
@@ -505,7 +506,7 @@ Lemma elim_stld_blocks_wfPI: forall los nts fh dones (pinfo:PhiInfo) f0 dones0
      wf_system
        [module_intro los nts
          (Ps1 ++ product_fdef (fdef_intro fh bs) :: Ps2)]),
-  WF_PhiInfo (update_pinfo pinfo f0).
+  exists pinfo', WF_PhiInfo pinfo' /\ keep_pinfo f0 pinfo pinfo'.
 Proof.
   intros.
   rewrite_env (nil ++ bs) in HwfS.
@@ -562,6 +563,76 @@ Proof.
     destruct flag0; auto.
 Qed.
 
+Lemma keep_pinfo_trans: forall f f' p1 p2 p3
+  (H1: keep_pinfo f p1 p2) (H2: keep_pinfo f' p2 p3),
+  keep_pinfo f' p1 p3.
+Proof.
+  intros.
+  destruct H1 as [A [B [C D]]].
+  destruct H2 as [A' [B' [C' D']]].
+  repeat split; try solve [auto | etransitivity; eauto].
+Qed.
+
+Lemma change_keep_pinfo: forall f pinfo1 pinfo2
+  (H1: PI_id pinfo1 = PI_id pinfo2)
+  (H2: PI_typ pinfo1 = PI_typ pinfo2)
+  (H3: PI_align pinfo1 = PI_align pinfo2),
+  (exists pinfo' : PhiInfo, WF_PhiInfo pinfo' /\ keep_pinfo f pinfo1 pinfo') -> 
+  exists pinfo' : PhiInfo, WF_PhiInfo pinfo' /\ keep_pinfo f pinfo2 pinfo'.
+Proof.
+  intros.
+  destruct H as [A [B C]].
+  exists A. split; auto.
+  unfold keep_pinfo in *.
+  rewrite <- H1. rewrite <- H2. rewrite <- H3. auto.
+Qed.
+
+Lemma update_pinfo_refl: forall f0 pinfo pinfo' 
+  (Hkp: keep_pinfo f0 pinfo pinfo'), (update_pinfo pinfo' f0) = pinfo'.
+Proof.
+  intros.
+  destruct Hkp as [EQ _]; subst. destruct pinfo'. auto.
+Qed.
+
+Ltac solve_keep_pinfo :=
+match goal with
+| Hkeep : keep_pinfo _ ?pinfo ?pinfo' |- PI_id ?pinfo' = PI_id ?pinfo =>
+  destruct Hkeep as [? [? ?]]; auto
+| Hkeep : keep_pinfo ?f ?pinfo ?pinfo' |- PI_f ?pinfo' = ?f =>
+  destruct Hkeep as [? ?]; auto
+| Hkeep : keep_pinfo ?f1 ?pinfo ?pinfo',
+  HeqR : exists _:_,
+            WF_PhiInfo _ /\ keep_pinfo ?f0 ?pinfo' _ |-
+  exists _:_, WF_PhiInfo _ /\ keep_pinfo ?f0 ?pinfo _ =>
+  let A:=fresh "A" in
+  destruct HeqR as [A [? ?]];
+  exists A; split; auto; apply keep_pinfo_trans with (f:=f1)(p2:=pinfo'); auto
+| G: exists _:_, WF_PhiInfo _ /\ keep_pinfo ?f (update_pinfo ?pi _) _ |-
+  exists _:_, WF_PhiInfo _ /\ keep_pinfo ?f ?pi _ =>
+  let A:=fresh "A" in
+  destruct G as [A [? ?]]; exists A; split; auto
+| pinfo := {|
+           PI_f := _;
+           PI_rd := _;
+           PI_id := ?pid;
+           PI_typ := _;
+           PI_num := _;
+           PI_align := _ |} : PhiInfo, 
+  Hkeep : keep_pinfo _ ?pinfo ?pinfo' |- PI_id ?pinfo' = ?pid =>
+  destruct Hkeep as [_ [? ?]]; auto
+| pinfo := {|
+           PI_f := _;
+           PI_rd := _;
+           PI_id := ?pid;
+           PI_typ := _;
+           PI_num := _;
+           PI_align := _ |} : PhiInfo, 
+  Hkeep : keep_pinfo _ ?pinfo ?pinfo' |- ?pid = PI_id ?pinfo' =>
+  destruct Hkeep as [_ [? ?]]; auto
+| H: ?f _ _ = ?e |- ?f _ _ = ?e => rewrite H; f_equal; solve_keep_pinfo
+| H: ?e = ?f _ _ |- ?f _ _ = ?e => rewrite H; f_equal; solve_keep_pinfo
+end.
+
 Lemma elim_stld_sim_wfS_wfPI: forall f1 dones1 f2 dones2 Ps1 Ps2 los nts main
   VarArgs pid (pinfo:PhiInfo)
   (Hpass: SafePrimIter.iterate _ (elim_stld_step pid)
@@ -573,7 +644,7 @@ Lemma elim_stld_sim_wfS_wfPI: forall f1 dones1 f2 dones2 Ps1 Ps2 los nts main
   (HwfS : wf_system S2) (Hok: defined_program S2 main VarArgs),
   (program_sim S1 S2 main VarArgs /\ wf_system S1 /\
     defined_program S1 main VarArgs) /\
-  WF_PhiInfo (update_pinfo pinfo f2).
+  exists pinfo', WF_PhiInfo pinfo' /\ keep_pinfo f2 pinfo pinfo'.
 Proof.
   intros. subst.
   set (P:=fun (re:(fdef * list id)) =>
@@ -586,11 +657,11 @@ Proof.
            defined_program 
             [module_intro los nts (Ps1 ++ product_fdef f :: Ps2)]
             main VarArgs) /\
-          WF_PhiInfo (update_pinfo pinfo f)
+          exists pinfo', WF_PhiInfo pinfo' /\ keep_pinfo f pinfo pinfo'
        ).
   assert (P (PI_f pinfo, dones1)) as HPf1.
     unfold P.
-    split; auto using program_sim_refl.
+    split; auto using program_sim_refl. instantiate_pinfo.
   apply SafePrimIter.iterate_prop with (P:=P) in Hpass; auto.
     unfold elim_stld_step.
     intros a HPa.
@@ -602,16 +673,16 @@ Proof.
     assert (P (f0, dones0)) as HPf0.
       unfold P.
       symmetry in HeqR.
-      destruct HPa as [[Hsima [HwfSa Hoka]] HwfPIa].
-      change (PI_id pinfo) with (PI_id (update_pinfo pinfo (fdef_intro fh bs)))
-        in HeqR.
+      destruct HPa as 
+        [[Hsima [HwfSa Hoka]] [pinfo' [HwfPIa Hkeep]]].
+      replace (PI_id pinfo) with (PI_id pinfo') in HeqR; try solve_keep_pinfo.
       split.
         apply program_sim_wfS_trans with (P2:=
                 [module_intro los nts
                  (Ps1 ++ product_fdef (fdef_intro fh bs) :: Ps2)]); auto.
           intros.
-          eapply elim_stld_blocks_sim_wfS in HeqR; eauto.
-        eapply elim_stld_blocks_wfPI in HeqR; eauto.
+          eapply elim_stld_blocks_sim_wfS in HeqR; eauto; try solve_keep_pinfo.
+        eapply elim_stld_blocks_wfPI in HeqR; eauto; try solve_keep_pinfo.
 
     destruct flag0; auto.
 Qed.
@@ -714,29 +785,29 @@ Proof.
 
             apply phinodes_placement_successors.
 
-    assert (WF_PhiInfo (update_pinfo pinfo f0)) as HwfPIf0.
-      change (update_pinfo pinfo f0) with
-             (update_pinfo
+    assert (exists pinfo', WF_PhiInfo pinfo' /\ keep_pinfo f0 pinfo pinfo') 
+      as HwfPIf0.
+     apply change_keep_pinfo with (pinfo1:=
                (update_pinfo pinfo
                  (phinodes_placement rd pid ty al (successors f)
-                   (make_predecessors (successors f)) f)) f0).
+                   (make_predecessors (successors f)) f))); auto.
      destruct HPa as [HPa1 [HPa2 HPa3]].
      eapply elim_stld_sim_wfS_wfPI; eauto.
        rewrite EQ1. auto.
        eapply phinodes_placement_wfPI; eauto.
-         rewrite EQ1. simpl.
-         eapply phinodes_placement_wfS; eauto.
+       rewrite EQ1. simpl. eapply phinodes_placement_wfS; eauto.
        eapply program_sim__preserves__defined_program; eauto.
          rewrite EQ1. simpl.
          eapply phinodes_placement_sim; eauto.
 
+    destruct HwfPIf0 as [pinfo' [HwfPIf0 Hkeep]].
     assert (P (if load_in_fdef pid f0 then f0 else elim_dead_st_fdef pid f0,
               nil) /\
-            WF_PhiInfo (update_pinfo pinfo
+            WF_PhiInfo (update_pinfo pinfo'
               (if load_in_fdef pid f0 then f0 else elim_dead_st_fdef pid f0)))
       as HPf.
       remember (load_in_fdef pid f0) as R.
-      destruct R; auto.
+      destruct R; try solve [erewrite update_pinfo_refl; eauto 2].
       destruct HPf0 as [HPf0 HPf0'].
       split.
       Case "1".
@@ -746,11 +817,11 @@ Proof.
                   [module_intro los nts (Ps1 ++ product_fdef f0 :: Ps2)]); auto.
             intros.
             split.
-              eapply dse_sim with (pinfo:=mkPhiInfo f0 rd pid ty num al); eauto.
+              eapply dse_sim with (pinfo:=pinfo'); eauto; solve_keep_pinfo.
             split.
-              eapply dse_wfS with (pinfo:=mkPhiInfo f0 rd pid ty num al); eauto.
+              eapply dse_wfS with (pinfo:=pinfo'); eauto; solve_keep_pinfo.
               eapply program_sim__preserves__defined_program; eauto.
-                eapply dse_sim with (pinfo:=mkPhiInfo f0 rd pid ty num al); eauto.
+                eapply dse_sim with (pinfo:=pinfo'); eauto; solve_keep_pinfo.
         SCase "1.2".
           destruct HPf0' as [J1 J2].
           split.
@@ -761,16 +832,7 @@ Proof.
 
       Case "2".
         destruct HPf0 as [HPf00 [HPf01 HPf02]].
-        change (update_pinfo pinfo (elim_dead_st_fdef pid f0)) with
-                 (update_pinfo
-                   (update_pinfo
-                     (update_pinfo pinfo
-                       (phinodes_placement rd pid ty al (successors f)
-                         (make_predecessors (successors f)) f))
-                   f0)
-                   (elim_dead_st_fdef pid f0)
-                 ).
-        eapply dse_wfPI; eauto.
+        eapply dse_wfPI; eauto; solve_keep_pinfo.
 
     destruct HPf as [HPf HwfPI0].
     remember (used_in_fdef pid
@@ -778,6 +840,7 @@ Proof.
     destruct R; auto.
     destruct HPf as [HPf HPf'].
     split.
+    Case "1".
       apply program_sim_wfS_trans with (P2:=
                  [module_intro los nts
                    (Ps1 ++ product_fdef
@@ -786,20 +849,21 @@ Proof.
         intros.
         split.
           eapply dae_sim with
-            (pinfo:=mkPhiInfo
-              (if load_in_fdef pid f0 then f0 else elim_dead_st_fdef pid f0)
-              rd pid ty num al); eauto.
+            (pinfo:=update_pinfo pinfo'
+              (if load_in_fdef pid f0 then f0 else elim_dead_st_fdef pid f0)); eauto 1;
+            simpl; solve_keep_pinfo.
         split.
           eapply dae_wfS with
-            (pinfo:=mkPhiInfo
-              (if load_in_fdef pid f0 then f0 else elim_dead_st_fdef pid f0)
-              rd pid ty num al); eauto.
+            (pinfo:=update_pinfo pinfo'
+              (if load_in_fdef pid f0 then f0 else elim_dead_st_fdef pid f0)); eauto 1;
+            simpl; solve_keep_pinfo.
           eapply program_sim__preserves__defined_program; eauto.
             eapply dae_sim with
-              (pinfo:=mkPhiInfo
-                (if load_in_fdef pid f0 then f0 else elim_dead_st_fdef pid f0)
-                rd pid ty num al); eauto.
+              (pinfo:=update_pinfo pinfo'
+                (if load_in_fdef pid f0 then f0 else elim_dead_st_fdef pid f0)); eauto 1;
+            simpl; solve_keep_pinfo.
 
+    Case "2".
       destruct HPf' as [Hreach' Hsucc'].
       split.
         transitivity
